Proving Confidentiality, still grinding.

AbstractPlatform/MemConfidentialityProof.bpl
@@ -12,10 +12,6 @@ procedure ProveConfidentialityMem(
     modifies cache_valid_map, cache_tag_map;
     modifies cache_valid_map_1, cache_tag_map_1;
     modifies cache_valid_map_2, cache_tag_map_2;
-    modifies untrusted_addr_valid;
-    modifies untrusted_addr_map;
-    modifies untrusted_regs;
-    modifies untrusted_pc;
     modifies tap_enclave_metadata_valid;
     modifies tap_enclave_metadata_addr_map;
     modifies tap_enclave_metadata_addr_valid;
@@ -25,6 +21,8 @@ procedure ProveConfidentialityMem(
     modifies tap_enclave_metadata_regs;
     modifies tap_enclave_metadata_paused;
     modifies tap_enclave_metadata_cache_conflict;
+    modifies tap_enclave_metadata_privileged;
+    modifies tap_enclave_metadata_owner_map;
     modifies cpu_mem_1;
     modifies cpu_regs_1;
     modifies cpu_pc_1;
@@ -32,10 +30,6 @@ procedure ProveConfidentialityMem(
     modifies cpu_addr_valid_1;
     modifies cpu_addr_map_1;
     modifies cpu_owner_map_1;
-    modifies untrusted_addr_valid_1;
-    modifies untrusted_addr_map_1;
-    modifies untrusted_regs_1;
-    modifies untrusted_pc_1;
     modifies tap_enclave_metadata_valid_1;
     modifies tap_enclave_metadata_addr_map_1;
     modifies tap_enclave_metadata_addr_valid_1;
@@ -45,6 +39,8 @@ procedure ProveConfidentialityMem(
     modifies tap_enclave_metadata_regs_1;
     modifies tap_enclave_metadata_paused_1;
     modifies tap_enclave_metadata_cache_conflict_1;
+    modifies tap_enclave_metadata_privileged_1;
+    modifies tap_enclave_metadata_owner_map_1;
     modifies cpu_mem_2;
     modifies cpu_regs_2;
     modifies cpu_pc_2;
@@ -52,10 +48,6 @@ procedure ProveConfidentialityMem(
     modifies cpu_addr_valid_2;
     modifies cpu_addr_map_2;
     modifies cpu_owner_map_2;
-    modifies untrusted_addr_valid_2;
-    modifies untrusted_addr_map_2;
-    modifies untrusted_regs_2;
-    modifies untrusted_pc_2;
     modifies tap_enclave_metadata_valid_2;
     modifies tap_enclave_metadata_addr_map_2;
     modifies tap_enclave_metadata_addr_valid_2;
@@ -65,6 +57,8 @@ procedure ProveConfidentialityMem(
     modifies tap_enclave_metadata_regs_2;
     modifies tap_enclave_metadata_paused_2;
     modifies tap_enclave_metadata_cache_conflict_2;
+    modifies tap_enclave_metadata_privileged_2;
+    modifies tap_enclave_metadata_owner_map_2;
 {
     var eid, r_eid                                   : tap_enclave_id_t;
     var status, status_1, status_2                   : enclave_op_result_t;
@@ -74,8 +68,9 @@ procedure ProveConfidentialityMem(
     var e_excl_map                                   : excl_map_t;
     var e_container_data_1, e_container_data_2       : container_data_t;
     var e_entrypoint_1, e_entrypoint_2               : vaddr_t;
+    var e_privileged_1, e_privileged_2               : bool;
     var current_mode, current_mode_1, current_mode_2 : mode_t;
-    var enclave_dead, enclave_dead_1, enclave_dead_2 : bool;
+    // var enclave_dead, enclave_dead_1, enclave_dead_2 : bool;
     var observation_1, observation_2                 : word_t;
     var e_proof_op, r_proof_op                       : tap_proof_op_t;
     var word_1, word_2                               : word_t;
@@ -113,9 +108,9 @@ procedure ProveConfidentialityMem(
     assert cpu_owner_map[cpu_addr_map[cpu_pc]] == cpu_enclave_id;
     assert cpu_enclave_id == tap_null_enc_id;
     // initialize the untrusted (OS) state with sane values.
-    untrusted_addr_valid := cpu_addr_valid;
-    untrusted_addr_map := cpu_addr_map;
-    untrusted_pc := cpu_pc;
+    tap_enclave_metadata_addr_valid[tap_null_enc_id] := cpu_addr_valid;
+    tap_enclave_metadata_addr_map[tap_null_enc_id] := cpu_addr_map;
+    tap_enclave_metadata_pc[tap_null_enc_id] := cpu_pc;
 
     // create two copies of state.
     call SaveContext_1();
@@ -127,7 +122,7 @@ procedure ProveConfidentialityMem(
     call RestoreContext_1();
     call InitOSMem(e_excl_map, e_container_data_1);
     call status := launch(eid, e_addr_valid_1, e_addr_map_1, 
-                          e_excl_vaddr_1, e_excl_map, e_entrypoint_1);
+                          e_excl_vaddr_1, e_excl_map, e_entrypoint_1, e_privileged_1);
     assume tap_enclave_metadata_cache_conflict[eid] == cache_conflict;
     assume status == enclave_op_success;
     call SaveContext_1();
@@ -135,7 +130,7 @@ procedure ProveConfidentialityMem(
     call RestoreContext_2();
     call InitOSMem(e_excl_map, e_container_data_2);
     call status := launch(eid, e_addr_valid_2, e_addr_map_2, 
-                          e_excl_vaddr_2, e_excl_map, e_entrypoint_2);
+                          e_excl_vaddr_2, e_excl_map, e_entrypoint_2, e_privileged_2);
     assume status == enclave_op_success;
     assume tap_enclave_metadata_cache_conflict[eid] == cache_conflict;
     call SaveContext_2();
@@ -148,11 +143,78 @@ procedure ProveConfidentialityMem(
     observation_2 := k0_word_t;
 
     current_mode := mode_untrusted;
-    while (!enclave_dead)
-        //// The property ////
+    current_mode_1 := current_mode;
+    current_mode_2 := current_mode;
+
+    while (*)
+        // M adversary: unconditionally
         invariant (observation_1 == observation_2);
         //// General invariants /////
-        invariant current_mode == mode_untrusted || current_mode == mode_enclave;
+        invariant !tap_enclave_metadata_privileged_1[tap_null_enc_id];
+        invariant !tap_enclave_metadata_privileged_2[tap_null_enc_id];
+
+        //  privileged relationship: unique PE
+        invariant ( e_privileged_1) ==> (forall e : tap_enclave_id_t :: (tap_enclave_metadata_valid_1[e]) ==> 
+                (tap_enclave_metadata_privileged_1[e] <==> e == eid));
+        invariant (!e_privileged_1) ==> (forall e : tap_enclave_id_t :: (tap_enclave_metadata_valid_1[e]) ==> 
+                (!tap_enclave_metadata_privileged_1[e]));
+        invariant ( e_privileged_2) ==> (forall e : tap_enclave_id_t :: (tap_enclave_metadata_valid_2[e]) ==> 
+                (tap_enclave_metadata_privileged_2[e] <==> e == eid));
+        invariant (!e_privileged_2) ==> (forall e : tap_enclave_id_t :: (tap_enclave_metadata_valid_2[e]) ==> 
+                (!tap_enclave_metadata_privileged_2[e]));
+
+        // valid guarantee
+        invariant tap_enclave_metadata_valid_1[tap_null_enc_id];
+        invariant tap_enclave_metadata_valid_2[tap_null_enc_id];
+        invariant (forall e : tap_enclave_id_t :: 
+                    special_enclave_id(e) ==> !tap_enclave_metadata_valid_1[e]);
+        invariant (forall e: tap_enclave_id_t :: 
+                    special_enclave_id(e) ==> !tap_enclave_metadata_valid_2[e]);
+
+        // enclave ownermap relationship: valid enclave's parent must be valid
+        invariant (forall e : tap_enclave_id_t :: tap_enclave_metadata_valid_1[e] ==>
+                    (tap_enclave_metadata_valid_1[tap_enclave_metadata_owner_map_1[e]]));
+        invariant (forall e : tap_enclave_id_t :: tap_enclave_metadata_valid_2[e] ==> 
+                    (tap_enclave_metadata_valid_2[tap_enclave_metadata_owner_map_2[e]]));
+
+        // enclave ownermap relationship: special children
+        invariant tap_enclave_metadata_owner_map_1[eid] == tap_null_enc_id;
+        invariant tap_enclave_metadata_owner_map_2[eid] == tap_null_enc_id;
+        invariant tap_enclave_metadata_owner_map_1[tap_null_enc_id] == tap_null_enc_id;
+        invariant tap_enclave_metadata_owner_map_2[tap_null_enc_id] == tap_null_enc_id;
+
+        // enclave ownermap relationship: the maximal parent-tree depth is 2 
+        invariant (forall e : tap_enclave_id_t :: (tap_enclave_metadata_valid_1[e]) ==> 
+                    (tap_enclave_metadata_owner_map_1[tap_enclave_metadata_owner_map_1[e]] == tap_null_enc_id));
+        invariant (forall e : tap_enclave_id_t :: (tap_enclave_metadata_valid_2[e]) ==> 
+                    (tap_enclave_metadata_owner_map_2[tap_enclave_metadata_owner_map_2[e]] == tap_null_enc_id));
+
+        // enclave ownermap relationship: enclave with chidren must be privileged 
+        invariant (forall e : tap_enclave_id_t :: 
+                    (tap_enclave_metadata_valid_1[e] && tap_enclave_metadata_owner_map_1[e] != tap_null_enc_id) ==> 
+                        (tap_enclave_metadata_privileged_1[tap_enclave_metadata_owner_map_1[e]]));
+        invariant (forall e : tap_enclave_id_t :: 
+                    (tap_enclave_metadata_valid_2[e] && tap_enclave_metadata_owner_map_2[e] != tap_null_enc_id) ==> 
+                        (tap_enclave_metadata_privileged_2[tap_enclave_metadata_owner_map_2[e]]));
+        
+        // extend the exclusive-memory consistency to PE and NE children.
+        // 1.   constrain this consistency to PE-controlled enclave.
+        invariant (forall e : tap_enclave_id_t, v : vaddr_t :: 
+                    (tap_enclave_metadata_valid_1[e] && (tap_enclave_metadata_privileged_1[e] || tap_enclave_metadata_privileged_1[tap_enclave_metadata_owner_map_1[e]]) ==> 
+                        (tap_enclave_metadata_addr_excl_1[e][v] <==> cpu_owner_map_1[tap_enclave_metadata_addr_map_1[e][v]] == e)));
+        invariant (forall e : tap_enclave_id_t, v : vaddr_t :: 
+                    (tap_enclave_metadata_valid_2[e] && (tap_enclave_metadata_privileged_2[e] || tap_enclave_metadata_privileged_2[tap_enclave_metadata_owner_map_2[e]]) ==> 
+                        (tap_enclave_metadata_addr_excl_2[e][v] <==> cpu_owner_map_2[tap_enclave_metadata_addr_map_2[e][v]] == e)));
+        // 2.   constraint this consistency to PE.
+        invariant (forall v : vaddr_t :: 
+                    (tap_enclave_metadata_privileged_1[cpu_enclave_id_1] || tap_enclave_metadata_privileged_1[tap_enclave_metadata_owner_map_1[cpu_enclave_id_1]]) ==> 
+                        (tap_enclave_metadata_addr_excl_1[cpu_enclave_id_1][v] <==> cpu_owner_map_1[cpu_addr_map_1[v]] == cpu_enclave_id_1));
+        invariant (forall v : vaddr_t :: 
+                    (tap_enclave_metadata_privileged_2[cpu_enclave_id_2] || tap_enclave_metadata_privileged_2[tap_enclave_metadata_owner_map_2[cpu_enclave_id_2]]) ==> 
+                        (tap_enclave_metadata_addr_excl_2[cpu_enclave_id_2][v] <==> cpu_owner_map_2[cpu_addr_map_2[v]] == cpu_enclave_id_2));
+        
+        invariant current_mode_1 == mode_untrusted || current_mode_1 == mode_enclave;
+        invariant current_mode_2 == mode_untrusted || current_mode_2 == mode_untrusted;
         // memory is not assigned to an enclave that doesn't exist.
         invariant (forall pa : wap_addr_t, e : tap_enclave_id_t ::
                     (valid_enclave_id(e) && !tap_enclave_metadata_valid_1[e]) ==> 
@@ -167,84 +229,102 @@ procedure ProveConfidentialityMem(
                     !valid_enclave_id(e) ==> !tap_enclave_metadata_valid_1[tap_null_enc_id]);
         invariant (forall e : tap_enclave_id_t ::
                     !valid_enclave_id(e) ==> !tap_enclave_metadata_valid_2[tap_null_enc_id]);
-        invariant (current_mode == mode_untrusted) ==> cpu_enclave_id_1 != eid;
-        invariant (current_mode == mode_untrusted) ==> cpu_enclave_id_2 != eid;
-        invariant (current_mode == mode_enclave) ==> (cpu_enclave_id_1 == eid);
-        invariant (current_mode == mode_enclave) ==> (cpu_enclave_id_2 == eid);
+        invariant (current_mode_1 == mode_untrusted) ==> cpu_enclave_id_1 != eid;
+        invariant (current_mode_2 == mode_untrusted) ==> cpu_enclave_id_2 != eid;
+        invariant (current_mode_1 == mode_enclave) ==> (cpu_enclave_id_1 == eid);
+        invariant (current_mode_2 == mode_enclave) ==> (cpu_enclave_id_2 == eid);
         //-------------------------------------------------------------------//
         // Enclave 'eid' is mostly alive                                     //
         //-------------------------------------------------------------------//
         invariant (valid_enclave_id(eid));
         invariant (cpu_enclave_id_1 != tap_blocked_enc_id);
         invariant (cpu_enclave_id_2 != tap_blocked_enc_id);
-        invariant (!enclave_dead ==> tap_enclave_metadata_valid_1[eid]);
-        invariant (!enclave_dead ==> tap_enclave_metadata_valid_2[eid]);
+        invariant (tap_enclave_metadata_valid_1[eid]);
+        invariant (tap_enclave_metadata_valid_2[eid]);
         // maintain invariants about excl_vaddr.
-        invariant (!enclave_dead) ==>
-                        (tap_enclave_metadata_addr_excl_1[eid] == e_excl_vaddr_1);
-        invariant (!enclave_dead) ==>
-                        (tap_enclave_metadata_addr_excl_2[eid] == e_excl_vaddr_2);
+        invariant tap_enclave_metadata_addr_excl_1[eid] == e_excl_vaddr_1;
+        invariant tap_enclave_metadata_addr_excl_2[eid] == e_excl_vaddr_2;
         // invariants about addr_map
         invariant (forall v : vaddr_t ::
-                      (!enclave_dead && e_excl_vaddr_1[v]) ==>
-                          (tap_enclave_metadata_addr_map_1[eid][v] == e_addr_map_1[v]));
+                      e_excl_vaddr_1[v] ==>
+                          tap_enclave_metadata_addr_map_1[eid][v] == e_addr_map_1[v]);
         invariant (forall v : vaddr_t ::
-                      (!enclave_dead && e_excl_vaddr_2[v]) ==>
-                          (tap_enclave_metadata_addr_map_2[eid][v] == e_addr_map_2[v]));
+                      e_excl_vaddr_2[v] ==>
+                          tap_enclave_metadata_addr_map_2[eid][v] == e_addr_map_2[v]);
         // invariants about e_excl_addr
         invariant (forall p : wap_addr_t :: 
-                    (!enclave_dead) ==> ((cpu_owner_map_1[p] == eid) <==> e_excl_map[p]));
+                    (cpu_owner_map_1[p] == eid) <==> e_excl_map[p]);
         invariant (forall p : wap_addr_t :: 
-                    (!enclave_dead) ==> ((cpu_owner_map_2[p] == eid) <==> e_excl_map[p]));
+                    (cpu_owner_map_2[p] == eid) <==> e_excl_map[p]);
         invariant (forall v : vaddr_t, p : wap_addr_t :: 
-                        (!enclave_dead && e_excl_vaddr_1[v] && p == e_addr_map_1[v])
+                        (e_excl_vaddr_1[v] && p == e_addr_map_1[v])
                             ==> e_excl_map[p]);
         invariant (forall v : vaddr_t, p : wap_addr_t :: 
-                        (!enclave_dead && e_excl_vaddr_2[v] && p == e_addr_map_2[v])
+                        (e_excl_vaddr_2[v] && p == e_addr_map_2[v])
                             ==> e_excl_map[p]);
         //-------------------------------------------------------------------//
         // Now deal with the enclaves.
         //-------------------------------------------------------------------//
         invariant (forall v : vaddr_t ::
-                    (current_mode == mode_enclave && e_excl_vaddr_1[v]) ==> 
+                    (current_mode_1 == mode_enclave && e_excl_vaddr_1[v]) ==> 
                         (cpu_addr_map_1[v] == e_addr_map_1[v]));
         invariant (forall v : vaddr_t ::
-                    (current_mode == mode_enclave && e_excl_vaddr_2[v]) ==> 
+                    (current_mode_2 == mode_enclave && e_excl_vaddr_2[v]) ==> 
                         (cpu_addr_map_2[v] == e_addr_map_2[v]));
         //-------------------------------------------------------------------//
         // CPU state is the same                                             //
         //-------------------------------------------------------------------//
-        // same PC.
-        invariant (current_mode == mode_untrusted) ==> (cpu_pc_1 == cpu_pc_2);
-        // same mode of operation.
-        invariant (cpu_enclave_id_1 == cpu_enclave_id_2);
-        // same regs.
-        invariant (current_mode == mode_untrusted) ==> (cpu_regs_1 == cpu_regs_2);
-        // same va->pa.
-        invariant (current_mode == mode_untrusted) ==> 
-                    (cpu_addr_valid_1 == cpu_addr_valid_2);
-        invariant (current_mode == mode_untrusted) ==> 
-                    (cpu_addr_map_1 == cpu_addr_map_2);
-        // owner map is the same.
-        invariant (forall pa : wap_addr_t :: (cpu_owner_map_1[pa] == cpu_owner_map_2[pa]));
-        // memory is the same except for the enclave memory.
-        invariant (forall pa : wap_addr_t :: !e_excl_map[pa] ==> (cpu_mem_1[pa] == cpu_mem_2[pa]));
+        // TODO: This should be further checked. Whether this condition lead to observation results.
+        // Apr 16, 2023.
+        invariant (e_privileged_1 == e_privileged_2) ==> (current_mode_1 == current_mode_2);
+
+        // Harmonized case.
+        invariant (e_privileged_1 == e_privileged_2) ==> 
+            ((current_mode_1 == mode_untrusted) ==> (cpu_pc_1 == cpu_pc_2));
+        invariant (e_privileged_1 == e_privileged_2) ==> 
+            ((current_mode_1 == mode_untrusted) ==> (cpu_regs_1 == cpu_regs_2));
+        invariant (e_privileged_1 == e_privileged_2) ==> 
+            ((current_mode_1 == mode_untrusted) ==> (cpu_addr_valid_1 == cpu_addr_valid_2));
+        invariant (e_privileged_1 == e_privileged_2) ==> 
+            ((current_mode_1 == mode_untrusted) ==> (cpu_addr_valid_1 == cpu_addr_map_2));
+        invariant (e_privileged_1 == e_privileged_2) ==> 
+            (forall pa : wap_addr_t :: (cpu_owner_map_1[pa] == cpu_owner_map_2[pa]));
+        invariant (e_privileged_1 == e_privileged_2) ==> 
+            (forall pa : wap_addr_t :: !e_excl_map[pa] ==> (cpu_mem_1[pa] == cpu_mem_2[pa]));
+        // Chaos case.
+        // TODO.
+
         //-------------------------------------------------------------------//
         // OS state is the same                                              //
         //-------------------------------------------------------------------//
         // OS va->pa 
-        invariant (untrusted_addr_valid_1 == untrusted_addr_valid_2);
-        invariant (untrusted_addr_map_1 == untrusted_addr_map_2);
+        invariant (tap_enclave_metadata_addr_valid_1[tap_null_enc_id] == tap_enclave_metadata_addr_valid_2[tap_null_enc_id]);
+        invariant (tap_enclave_metadata_addr_map_1[tap_null_enc_id] == tap_enclave_metadata_addr_map_2[tap_null_enc_id]);
         // OS regs.
-        invariant (untrusted_regs_1 == untrusted_regs_2);
-        invariant (untrusted_pc_1 == untrusted_pc_2);
+        invariant (tap_enclave_metadata_regs_1[tap_null_enc_id] == tap_enclave_metadata_regs_2[tap_null_enc_id]);
+        invariant (tap_enclave_metadata_pc_1[tap_null_enc_id] == tap_enclave_metadata_pc_2[tap_null_enc_id]);
         //-------------------------------------------------------------------//
         // Enclave state is the same except for eid (mostly). Some it is the //
         // the same for eid as well (addr_map and addr_excl).                //
         //-------------------------------------------------------------------//
+        
         // valid is the same except for eid.
-        invariant (forall e : tap_enclave_id_t :: (e != eid) ==>
+        invariant (e_privileged_1 == e_privileged_2) ==> 
+                (forall e : tap_enclave_id_t :: (e != eid) ==>
                     (tap_enclave_metadata_valid_1[e] == tap_enclave_metadata_valid_2[e]));
+
+        invariant (e_privileged_1 != e_privileged_2 && e_privileged_1) ==> 
+                (forall e : tap_enclave_id_t :: (e != eid && tap_enclave_metadata_owner_map_1[e] != eid) ==> 
+                    (tap_enclave_metadata_valid_1[e] == tap_enclave_metadata_valid_2[e]));
+
+        invariant (e_privileged_1 != e_privileged_2 && e_privileged_2) ==> 
+                (forall e : tap_enclave_id_t :: (e != eid && tap_enclave_metadata_owner_map_2[e] != eid) ==> 
+                    (tap_enclave_metadata_valid_1[e] == tap_enclave_metadata_valid_2[e]));
+        // invariant (forall e : tap_enclave_id_t :: (e != eid) ==>
+        //             (tap_enclave_metadata_valid_1[e] == tap_enclave_metadata_valid_2[e]));
+
+        // These same-check could also be adopted by chaos cases.
+        
         // addr valid is the same except for eid.
         invariant (forall e : tap_enclave_id_t :: 
                     (tap_enclave_metadata_valid_1[e] && tap_enclave_metadata_valid_2[e] && e != eid) ==>
@@ -275,6 +355,7 @@ procedure ProveConfidentialityMem(
                         (tap_enclave_metadata_paused_1[e] == tap_enclave_metadata_paused_2[e]));
     {
         if (current_mode == mode_untrusted) {
+            assume false;
             havoc r_proof_op, r_eid, r_pc, r_read, r_write, r_data, 
                   l_vaddr, s_vaddr, s_data, r_pt_eid, r_pt_va, 
                   pt_eid, pt_vaddr, pt_valid, pt_paddr, r_addr_valid, 
@@ -315,11 +396,18 @@ procedure ProveConfidentialityMem(
 
             // some sanity checks.
             assert status_1 == status_2;
+            
+            // Same mode is not guanranteed.
+            // case 1. untrusted - untrusted    -- do observation
+            // case 2. enclave - enclave        -- do different things
+            // case 3. unt - encl / encl - unt  -- encl do anything, unt do nothing or exit/pause
             assert current_mode_1 == current_mode_2;
-            assert enclave_dead_1 == enclave_dead_2;
+            // Considering deprecate enclave dead.
+            // assert enclave_dead_1 == enclave_dead_2;
+            // enclave_dead := enclave_dead_2;
             current_mode := current_mode_1;
-            enclave_dead := enclave_dead_2;
         } else {
+            assume false;
             havoc e_proof_op;
             assume tap_proof_op_valid_in_enclave(e_proof_op);
 
@@ -334,7 +422,8 @@ procedure ProveConfidentialityMem(
             call current_mode_2, load_addr_2, l_way, store_addr_2, store_data_2, s_way := 
                             EnclaveStep(current_mode, eid, e_proof_op);
             call SaveContext_2();
-
+            // This assumption should be adjusted.
+            // Ganxiang Yang @ Apr 16, 2023.
             assume (!e_excl_vaddr_1[load_addr_1] || !e_excl_vaddr_2[load_addr_2]) ==>
                    ((load_addr_1 == load_addr_2) && 
                     (cpu_addr_map_1[load_addr_1] == cpu_addr_map_2[load_addr_2]));
